Convert SinglyLinkedListWithRecursion to the style of the rest of the library

src/linear/implementation/SinglyLinkedListWithRecursion.dfy
@@ -1,9 +1,9 @@
 include "../../../src/Utils.dfy"
 
-class NonEmpty<A> {
+class Node {
   ghost var repr: set<object>;
-  var data: A;
-  var next: NonEmpty?<A>;
+  var data: int;
+  var next: Node?;
 
   predicate Valid()
     reads this, repr
@@ -20,7 +20,7 @@ class NonEmpty<A> {
       )
   }
 
-  predicate ValidUntil(n: NonEmpty<A>)
+  predicate ValidUntil(n: Node)
     reads this, repr
   {
     && this in repr
@@ -37,7 +37,7 @@ class NonEmpty<A> {
       )
   }
 
-  constructor(d: A)
+  constructor(d: int)
     ensures Valid()
     ensures fresh(repr - {this})
     ensures data == d
@@ -48,271 +48,298 @@ class NonEmpty<A> {
     next := null;
   }
 
-  predicate IsPrevOf(n: NonEmpty<A>)
+  predicate IsPrevOf(n: Node)
     reads this
   {
     next == n
   }
 
-  predicate IsBefore(n: NonEmpty<A>)
+  predicate IsBefore(n: Node)
     reads this
   {
     n in repr
   }
 }
 
-type List<A> = NonEmpty?<A>
-
-function Repr<A>(xs: List<A>): set<object>
-  reads xs
-{
-  if xs == null then
-    {}
-  else
-    xs.repr
-}
-
-predicate Valid<A>(xs: List<A>)
-  reads xs, Repr(xs)
-{
-  xs != null ==> xs.Valid()
-}
-
-function Model<A>(node: List<A>): seq<A>
-  reads node, Repr(node)
-  decreases Repr(node)
-  requires Valid(node)
+function ReprAux(node: Node?): set<object>
+  reads node
 {
   if node == null then
-    []
+    {}
   else
-    assert node.Valid();
-    assert node.next != null ==> node.next.Valid();
-    [node.data] + Model(node.next)
+    node.repr
 }
 
-function Head<A>(xs: NonEmpty<A>): A
-  reads xs, xs.repr
-  requires xs.Valid()
-  ensures Head(xs) == Model(xs)[0]
+predicate ValidAux(node: Node?)
+  reads node, ReprAux(node)
 {
-  xs.data
+  node != null ==> node.Valid()
 }
 
-function Tail<A>(xs: NonEmpty<A>): List<A>
-  reads xs, xs.repr
-  requires xs.Valid()
-  ensures Valid(Tail(xs))
-  ensures Model(Tail(xs)) == Model(xs)[1..]
-  ensures Repr(Tail(xs)) <= Repr(xs) - {xs}
-{
-  xs.next
-}
+class SinglyLinkedListWithRecursion {
+  var head: Node?
 
-method Cons<A>(x: A, xs: List<A>) returns (res: NonEmpty<A>)
-  requires xs != null ==> xs.Valid()
-  ensures res.Valid()
-  ensures Model(res) == [x] + Model(xs)
-  ensures fresh(Repr(res) - Repr(xs))
-  ensures Repr(res) >= Repr(xs)
-{
-  res := new NonEmpty(x);
-  res.next := xs;
-  if res.next != null {
-    res.repr := {res} + res.next.repr;
-  }
-}
-
-method Append<A>(xs: List<A>, ys: List<A>) returns (res: List<A>)
-  decreases Repr(xs)
-  requires Valid(xs)
-  requires Valid(ys)
-  ensures Valid(res)
-  ensures Model(res) == Model(xs) + Model(ys)
-{
-  if xs == null {
-    res := ys;
-  } else {
-    res := Append(xs.next, ys);
-    res := Cons(xs.data, res);
-  }
-}
-
-method ReverseAux<A>(xs: NonEmpty<A>, ys: List<A>)
-  returns (xs_: List<A>, ys_: NonEmpty<A>)
-  modifies xs, xs.repr
-
-  requires Valid(xs) && Valid(ys)
-  ensures Valid(xs_) && Valid(ys_)
-
-  requires Repr(xs) !! Repr(ys)
-  ensures Repr(xs_) !! Repr(ys_)
-
-  ensures old(Repr(xs)) + old(Repr(ys)) == Repr(xs_) + Repr(ys_)
-  ensures old(Repr(xs)) > Repr(xs_)
-  ensures Seq.Rev(old(Model(xs))) + old(Model(ys)) == Seq.Rev(Model(xs_)) + Model(ys_)
-{
-  xs_ := xs.next;
-  ys_ := xs;
-  ys_.next := ys;
-  ys_.repr := Repr(ys) + {ys_};
-}
-
-method Reverse<A>(xs: List<A>) returns (res: List<A>)
-  modifies xs, Repr(xs)
-  requires Valid(xs)
-  ensures Valid(res)
-  ensures old(Repr(xs)) == Repr(res)
-  ensures Seq.Rev(old(Model(xs))) == Model(res)
-{
-  var aux := xs;
-  res := null;
-  while aux != null
-    decreases Repr(aux)
-    invariant Repr(aux) !! Repr(res)
-    invariant Valid(aux)
-    invariant Valid(res)
-    invariant old(Repr(xs)) == Repr(aux) + Repr(res)
-    invariant Seq.Rev(old(Model(xs))) == Seq.Rev(Model(aux)) + Model(res)
+  function Repr(): set<object>
+    reads this, head
   {
-    aux, res := ReverseAux(aux, res);
+    if head == null then
+      {}
+    else
+      head.repr
   }
-}
 
-function PrevNode<A>(head: NonEmpty<A>, mid: NonEmpty<A>):
-    (prev: NonEmpty<A>)
-  decreases Repr(head)
-  reads head, head.repr, mid, mid.repr
-  requires mid in head.repr
-  requires head.ValidUntil(mid)
-  requires head != mid
-  ensures prev.next == mid
-  ensures head.ValidUntil(prev)
-{
-  if head.next == mid then
-    head
-  else
-    PrevNode(head.next, mid)
-}
-
-lemma ValidUntilFromValid<A>(head: NonEmpty<A>, mid: NonEmpty<A>)
-  decreases Repr(head)
-  requires mid in head.repr
-  requires head.Valid()
-  ensures head.ValidUntil(mid) && mid.Valid()
-{
-  if head != mid && head.next != null {
-    ValidUntilFromValid(head.next, mid);
+  predicate Valid()
+    reads this, head, Repr()
+  {
+    head != null ==> head.Valid()
   }
-}
 
-ghost method Repair(prevs: seq<NonEmpty<int>>, mid: List<int>)
-  modifies set n | n in multiset(prevs) :: n`repr
-  requires mid !in multiset(prevs)
-  requires forall n | n in prevs :: n !in Repr(mid)
-  requires forall i, j | 0 <= i < j < |prevs| :: prevs[i] != prevs[j]
-  requires forall i | 0 <= i < |prevs|-1 :: prevs[i].next == prevs[i+1]
-  requires prevs != [] ==> prevs[|prevs|-1].next == mid
-  requires Valid(mid)
-  ensures Valid(mid)
-  ensures forall n | n in multiset(prevs) :: n.Valid()
-{
-  if prevs != [] {
-    var prev := prevs[|prevs|-1];
-    assert prev in multiset(prevs);
-    prev.repr := {prev} + Repr(mid);
-    assert prevs == prevs[..|prevs|-1] + prevs[|prevs|-1..|prevs|];
-    assert multiset(prevs[..|prevs|-1]) <= multiset(prevs);
-    Repair(prevs[..|prevs|-1], prev);
-  }
-}
-
-lemma IsBeforeStepRight<A>(a: NonEmpty<A>, b: NonEmpty<A>)
-  decreases a.repr
-  requires Valid(a)
-  requires Valid(b)
-  requires b.next != null
-  requires a.IsBefore(b)
-  ensures a.IsBefore(b.next)
-{
-  if a != b && a.next != b {
-    IsBeforeStepRight(a.next, b);
-  }
-}
-
-lemma IsBeforeSubset<A>(a: NonEmpty<A>, b: NonEmpty<A>)
-  decreases a.repr
-  requires Valid(a)
-  requires Valid(b)
-  requires a.IsBefore(b)
-  ensures a.repr >= b.repr
-{
-  if a != b {
-    IsBeforeSubset(a.next, b);
-  }
-}
-
-lemma IsBeforeAntisym<A>(a: NonEmpty<A>, b: NonEmpty<A>)
-  decreases Repr(a)
-  requires Valid(a)
-  requires Valid(b)
-  requires a.IsBefore(b)
-  requires b.IsBefore(a)
-  ensures a == b
-{
-  if a != b && a.next != null {
-    IsBeforeStepRight(b, a);
-    IsBeforeAntisym(a.next, b);
-  }
-}
-
-function TakeSeq<A>(head: List<A>, mid: List<A>): (res: seq<NonEmpty<A>>)
-  decreases Repr(head)
-  reads Repr(head)
-  reads Repr(mid)
-  requires Valid(head)
-  requires Valid(mid)
-  requires mid in Repr(head)
-  ensures head != mid ==> head in res
-  ensures res != [] ==> res[0] == head && res[|res|-1].IsPrevOf(mid)
-  ensures forall n | n in res :: n in Repr(head)
-  ensures mid !in res
-  ensures forall n | n in multiset(res) :: n !in Repr(mid)
-  ensures forall i, j | 0 <= i < j < |res| :: res[i] != res[j]
-  ensures forall i | 0 <= i < |res|-1 :: res[i].IsPrevOf(res[i+1])
-  ensures res != [] ==> res[|res|-1].IsPrevOf(mid)
-{
-  if head == mid then
-    []
-  else
-    if head in Repr(mid) then
-      IsBeforeAntisym(head, mid);
-      assert head !in Repr(mid);
-      assert false;
+  static function ModelAux(node: Node?): seq<int>
+    reads node, ReprAux(node)
+    decreases ReprAux(node)
+    requires ValidAux(node)
+  {
+    if node == null then
       []
     else
-      assert head !in Repr(mid);
-      var res := [head] + TakeSeq(head.next, mid);
-      assert res != [] ==> res[0] == head && res[|res|-1].IsPrevOf(mid);
-      res
-}
+      assert ValidAux(node);
+      assert node.next != null ==> node.next.Valid();
+      [node.data] + ModelAux(node.next)
+  }
 
-method InPlaceInsert(head: NonEmpty<int>, mid: NonEmpty<int>, x: int)
-  modifies head, head.repr, mid, mid.repr
-  requires head != mid
-  requires head.Valid() && mid.Valid()
-  requires mid in head.repr
-  ensures head.Valid() && mid.Valid()
-{
-  var n := new NonEmpty(x);
-  ghost var prevs := TakeSeq(head, mid);
-  assert forall i | 0 <= i < |prevs|-1 :: prevs[i].IsPrevOf(prevs[i+1]);
-  assert prevs != [] ==> prevs[|prevs|-1].IsPrevOf(mid);
-  n.next := mid.next;
-  n.repr := Repr(mid.next) + {n};
-  mid.next := n;
-  mid.repr := {n} + mid.repr;
-  /*GHOST*/ Repair(prevs, mid);
-  assert Valid(head);
-  assert Valid(mid);
+  function Model(): seq<int>
+    reads this, head, Repr()
+    requires Valid()
+  {
+    ModelAux(head)
+  }
+
+  method Top() returns (x: int)
+    requires Valid()
+    requires Model() != []
+    ensures x == Model()[0]
+  {
+    x := head.data;
+  }
+
+  /*
+  function Tail(): List
+    reads xs, xs.repr
+    requires xs.Valid()
+    ensures Valid(Tail(xs))
+    ensures Model(Tail(xs)) == Model(xs)[1..]
+    ensures Repr(Tail(xs)) <= Repr(xs) - {xs}
+  {
+    xs.next
+  }
+  */
+
+  /*
+  method Cons(x: A, xs: List) returns (res: Node)
+    requires xs != null ==> xs.Valid()
+    ensures res.Valid()
+    ensures Model(res) == [x] + Model(xs)
+    ensures fresh(Repr(res) - Repr(xs))
+    ensures Repr(res) >= Repr(xs)
+  {
+    res := new Node(x);
+    res.next := xs;
+    if res.next != null {
+      res.repr := {res} + res.next.repr;
+    }
+  }
+
+  method Append(xs: List, ys: List) returns (res: List)
+    decreases Repr(xs)
+    requires Valid(xs)
+    requires Valid(ys)
+    ensures Valid(res)
+    ensures Model(res) == Model(xs) + Model(ys)
+  {
+    if xs == null {
+      res := ys;
+    } else {
+      res := Append(xs.next, ys);
+      res := Cons(xs.data, res);
+    }
+  }
+
+  method ReverseAux(xs: Node, ys: List)
+    returns (xs_: List, ys_: Node)
+    modifies xs, xs.repr
+
+    requires Valid(xs) && Valid(ys)
+    ensures Valid(xs_) && Valid(ys_)
+
+    requires Repr(xs) !! Repr(ys)
+    ensures Repr(xs_) !! Repr(ys_)
+
+    ensures old(Repr(xs)) + old(Repr(ys)) == Repr(xs_) + Repr(ys_)
+    ensures old(Repr(xs)) > Repr(xs_)
+    ensures Seq.Rev(old(Model(xs))) + old(Model(ys)) == Seq.Rev(Model(xs_)) + Model(ys_)
+  {
+    xs_ := xs.next;
+    ys_ := xs;
+    ys_.next := ys;
+    ys_.repr := Repr(ys) + {ys_};
+  }
+
+  method Reverse(xs: List) returns (res: List)
+    modifies xs, Repr(xs)
+    requires Valid(xs)
+    ensures Valid(res)
+    ensures old(Repr(xs)) == Repr(res)
+    ensures Seq.Rev(old(Model(xs))) == Model(res)
+  {
+    var aux := xs;
+    res := null;
+    while aux != null
+      decreases Repr(aux)
+      invariant Repr(aux) !! Repr(res)
+      invariant Valid(aux)
+      invariant Valid(res)
+      invariant old(Repr(xs)) == Repr(aux) + Repr(res)
+      invariant Seq.Rev(old(Model(xs))) == Seq.Rev(Model(aux)) + Model(res)
+    {
+      aux, res := ReverseAux(aux, res);
+    }
+  }
+  */
+
+  static function PrevNode(head: Node, mid: Node): (prev: Node)
+    decreases head.repr
+    reads head, head.repr, mid, mid.repr
+    requires mid in head.repr
+    requires head.ValidUntil(mid)
+    requires head != mid
+    ensures prev.next == mid
+    ensures head.ValidUntil(prev)
+  {
+    if head.next == mid then
+      head
+    else
+      PrevNode(head.next, mid)
+  }
+
+  static lemma ValidUntilFromValid(head: Node, mid: Node)
+    decreases head.repr
+    requires mid in head.repr
+    requires head.Valid()
+    ensures head.ValidUntil(mid) && mid.Valid()
+  {
+    if head != mid && head.next != null {
+      ValidUntilFromValid(head.next, mid);
+    }
+  }
+
+  ghost method Repair(prevs: seq<Node>, mid: Node?)
+    modifies set n | n in multiset(prevs) :: n`repr
+    requires mid !in multiset(prevs)
+    requires forall n | n in prevs :: n !in ReprAux(mid)
+    requires forall i, j | 0 <= i < j < |prevs| :: prevs[i] != prevs[j]
+    requires forall i | 0 <= i < |prevs|-1 :: prevs[i].next == prevs[i+1]
+    requires prevs != [] ==> prevs[|prevs|-1].next == mid
+    requires ValidAux(mid)
+    ensures ValidAux(mid)
+    ensures forall n | n in multiset(prevs) :: n.Valid()
+  {
+    if prevs != [] {
+      var prev := prevs[|prevs|-1];
+      assert prev in multiset(prevs);
+      prev.repr := {prev} + ReprAux(mid);
+      assert prevs == prevs[..|prevs|-1] + prevs[|prevs|-1..|prevs|];
+      assert multiset(prevs[..|prevs|-1]) <= multiset(prevs);
+      Repair(prevs[..|prevs|-1], prev);
+    }
+  }
+
+  lemma IsBeforeStepRight(a: Node, b: Node)
+    decreases a.repr
+    requires ValidAux(a)
+    requires ValidAux(b)
+    requires b.next != null
+    requires a.IsBefore(b)
+    ensures a.IsBefore(b.next)
+  {
+    if a != b && a.next != b {
+      IsBeforeStepRight(a.next, b);
+    }
+  }
+
+  lemma IsBeforeSubset(a: Node, b: Node)
+    decreases a.repr
+    requires ValidAux(a)
+    requires ValidAux(b)
+    requires a.IsBefore(b)
+    ensures a.repr >= b.repr
+  {
+    if a != b {
+      IsBeforeSubset(a.next, b);
+    }
+  }
+
+  lemma IsBeforeAntisym(a: Node, b: Node)
+    decreases ReprAux(a)
+    requires ValidAux(a)
+    requires ValidAux(b)
+    requires a.IsBefore(b)
+    requires b.IsBefore(a)
+    ensures a == b
+  {
+    if a != b && a.next != null {
+      IsBeforeStepRight(b, a);
+      IsBeforeAntisym(a.next, b);
+    }
+  }
+
+  function TakeSeq(head: Node, mid: Node): (res: seq<Node>)
+    decreases ReprAux(head)
+    reads ReprAux(head)
+    reads ReprAux(mid)
+    requires ValidAux(head)
+    requires ValidAux(mid)
+    requires mid in ReprAux(head)
+    ensures head != mid ==> head in res
+    ensures res != [] ==> res[0] == head && res[|res|-1].IsPrevOf(mid)
+    ensures forall n | n in res :: n in ReprAux(head)
+    ensures mid !in res
+    ensures forall n | n in multiset(res) :: n !in ReprAux(mid)
+    ensures forall i, j | 0 <= i < j < |res| :: res[i] != res[j]
+    ensures forall i | 0 <= i < |res|-1 :: res[i].IsPrevOf(res[i+1])
+    ensures res != [] ==> res[|res|-1].IsPrevOf(mid)
+  {
+    if head == mid then
+      []
+    else
+      if head in ReprAux(mid) then
+        IsBeforeAntisym(head, mid);
+        assert head !in ReprAux(mid);
+        assert false;
+        []
+      else
+        assert head !in ReprAux(mid);
+        var res := [head] + TakeSeq(head.next, mid);
+        assert res != [] ==> res[0] == head && res[|res|-1].IsPrevOf(mid);
+        res
+  }
+
+  method Insert(head: Node, mid: Node, x: int)
+    modifies head, head.repr, mid, mid.repr
+    requires head != mid
+    requires head.Valid() && mid.Valid()
+    requires mid in head.repr
+    ensures head.Valid() && mid.Valid()
+  {
+    var n := new Node(x);
+    ghost var prevs := TakeSeq(head, mid);
+    assert forall i | 0 <= i < |prevs|-1 :: prevs[i].IsPrevOf(prevs[i+1]);
+    assert prevs != [] ==> prevs[|prevs|-1].IsPrevOf(mid);
+    n.next := mid.next;
+    n.repr := ReprAux(mid.next) + {n};
+    mid.next := n;
+    mid.repr := {n} + mid.repr;
+    /*GHOST*/ Repair(prevs, mid);
+    assert ValidAux(head);
+    assert ValidAux(mid);
+  }
 }
